[arm] Fix accesses to the PC register.
On ARM, reading the PC gives a value that is a few bytes (usally 4 or 8 bytes) greater than the actual PC.

For now, we change all register reads to account for this, but in many cases the read may be provably unable to read the PC.  We could change those back to use the simpler reg function.

books/kestrel/arm/pseudocode.lisp
@@ -1190,3 +1190,31 @@
   (declare (xargs :guard (and (unsigned-byte-p 32 x)
                               (unsigned-byte-p 32 y))))
   (bvxor 32 x y))
+
+;;;;;;;;;;;;;;;;;;;;;;;;;;;;;;;;;;;;;;;;;;;;;;;;;;;;;;;;;;;;;;;;;;;;;;;;;;;;;;;;
+
+;; In the instruction semantic functions, access to register N must check
+;; whether N is *pc* and adjust by adding 8 (usually) if so.
+;todo: disable but need rules
+;; TODO: In some cases, this may be overkill because the register can't be the PC.
+;; In those cases, we could just use REG instead of REG*.
+(defun reg* (n arm)
+  (declare (xargs :guard (register-numberp n)
+                  :stobjs arm))
+  (let ((val (reg n arm)))
+    (if (equal *pc* n)
+        (let ((offset (if (equal (isetstate arm) *InstrSet_ARM*)
+                          8 ; todo: should this ever be 12?
+                        4 ; for Thumb (and ThumbEE)
+                        )))
+          (bvplus 32 offset val))
+      val)))
+
+(defthm unsigned-byte-p-of-reg*
+  (implies (and (<= 32 size)
+                (integerp size)
+                (< reg 16)
+                (natp reg)
+                (armp arm))
+           (unsigned-byte-p size (reg* reg arm)))
+  :hints (("Goal" :in-theory (enable reg*))))
